\documentclass[12pt]{article}
\usepackage{amsmath, amssymb, physics, geometry}
\usepackage{braket}
\geometry{a4paper, margin=1in}
\usepackage{hyperref}

\title{The Answer of Assignment 1}
\author{}
\date{}

\begin{document}

\maketitle

\begin{center}
    \textbf{Problem 1 Solution}
\end{center}

\textbf{(1)} From the eigenvalue equation $\hat{H}\psi(x) = h_n \psi(x)$ and the Hamiltonian operator $\hat{H} = -\frac{\hbar^2}{2m} \nabla^2$, we have:
\begin{align*}
    -\frac{\hbar^2}{2m} \nabla^2 \psi(x) = h_n \psi(x)
\end{align*}
The general solution is:
\begin{align*}
    \psi(x) = c_1 e^{w_1 x} + c_2 e^{w_2 x}, \quad w_1 = i\sqrt{\frac{2m h_n}{\hbar^2}}, \quad w_2 = -i\sqrt{\frac{2m h_n}{\hbar^2}}
\end{align*}
Given $p_n = \frac{2\pi\hbar n}{L}$, $h_n = \frac{2\pi^2 \hbar^2 n^2}{L m}$. Take $\psi_n(x) = e^{\frac{i p_n x}{\hbar}}$ as an example, the eigenvalue corresponding to $\ket{\psi_n}$ is $\frac{2\pi^2 \hbar^2 n^2}{L m}$.

\vspace{1em}
\textbf{(2)} 
\begin{align*}
    \braket{\psi_{n_1} | \psi_{n_2}} &= \int_{-\infty}^{+\infty} \psi_{n_1}^*(x)\, \psi_{n_2}(x) \, dx \\
    &= \int_{-\infty}^{+\infty} e^{-\frac{i p_{n_1} x}{\hbar}} e^{\frac{i p_{n_2} x}{\hbar}} dx \\
    &= \int_{-\infty}^{+\infty} e^{\frac{i (p_{n_2} - p_{n_1}) x}{\hbar}} dx \\
    &= \int_{-\infty}^{+\infty} e^{\frac{i 2\pi (n_2 - n_1)x}{L}} dx \\
    &= \lim_{l \to +\infty} \int_{-l}^{+l} e^{\frac{i 2\pi (n_2 - n_1)x}{L}} dx \\
    &= \lim_{l \to +\infty} \frac{L \sin\left[\frac{2\pi (n_2 - n_1) l}{L}\right]}{\pi (n_2 - n_1)}
\end{align*}
When $n_2 = n_1$, $\braket{\psi_{n_1} | \psi_{n_2}} \to \infty$ and
\begin{align*}
    \lim_{l \to +\infty} \int_{-\infty}^{+\infty} \frac{\sin(lx)}{x} dx = \pi
\end{align*}
So,
\begin{align*}
    \braket{\psi_{n_1} | \psi_{n_2}} = L \delta_{n_1 n_2}
\end{align*}
\textbf{(3)} 
When $L \to \infty$, $p_n$ becomes continuous and $\psi_n(x)$ becomes a plane wave.
\[
\braket{\psi_{p_1} | \psi_{p_2}} = \int_{-\infty}^{+\infty} e^{-\frac{i p_1 x}{\hbar}} e^{\frac{i p_2 x}{\hbar}} dx = \lim_{l \to +\infty} \frac{L \sin\left[\frac{(p_2 - p_1) l}{\hbar}\right]}{\pi (p_2 - p_1)} = L \delta(p_2 - p_1)
\]
\end{document}